\begin{proof}
	Let $\beta_1 = \sett{v_1,v_2,\cdots,v_n},v_1,v_2,\cdots,v_n \in W_1$,
		
		 $\beta_2 = \sett{u_1,u_2,\cdots,u_m},u_1,u_2,\cdots,u_m \in W_2$
		
		$W_1 + W_2 = \left\{\sum_{i=1}^n a_iv_i + \sum_{j=1}^{m}b_ju_j ~|~ a_1,\cdots,a_n,b_1,\cdots,b_m \in \mathcal{F}\,\right\} $
		\vspace*{0.2cm}
		
		\textbf{Claim : } $\spann{\beta_1 \cup \beta_2} \subseteq W_1 + W_2$
		
		let $x \in \spann{\beta_1 \cup \beta_2}~, x = a_1v_1 + a_2v_2 + \cdots + b_1u_1 + b_2u_2 + \cdots + b_mu_m$
		
		$\because W_1,W_2$ is a subspace of V $\therefore \sum^{n}_{i=1}a_iv_i \in W_1~,~ \sum^{m}_{i=1}b_iu_i \in W_2$
		
		$\therefore x \in W_1 + W_2,\spann{\beta_1 \cup \beta_2} \subseteq W_1 + W_2$
		
		\vspace*{0.3cm}
		\textbf{Claim.} $W_1 + W_2 \subseteq \spann{\beta_1 \cup \beta_2}$
		
		Let $x \in W_1 + W_2, x = (a_1v_1 + \cdots + a_nv_n) + (b_1u_1 + \cdots  + b_mu_m)$
		
		$\therefore x \in \spann{\beta_1 \cup \beta_2}$\ 
		$\therefore W_1 + W_2 \subseteq \spann{\beta_1 \cup \beta_2}$\ 
		$\therefore \spann{\beta_1 \cup \beta_2} = W_1 + W_2$

		
	    \vspace*{0.3cm}
		\textbf{Claim} ${\beta_1 \cup \beta_2}$ is linearly independent
		
		$\sum^n_{i=1}a_iv_1 + \sum^m_{j=1}b_ju_j = 0$ 
		$\implies\sum^n_{i_1}a_iv_i = -\sum^m_{j=1}b_ju_j$
		
		$\because \sum^n_{i=1}a_iv_i \in W_1~,~ -\sum^m_{j=1}b_ju_j \in W_2$ and $\sum^n_{i=1}a_iv_i~,~-\sum^m_{i=1}b_iu_i \in W_1 \cap W_2$ 
		
		$\because W_1 \cap W_2$ $\therefore \sum^n_{i=1}a_iv_i = -\sum^m_{j=1}b_ju_j = 0$ \ \ $\because \beta_1 , \beta_2$ is linearly independent
		
		$\therefore a_1 = \cdots = a_n = b_1=\cdots = b_m =0$ $\therefore \beta_1 \cup \beta_2$ is linearly independent
		
		$\therefore \beta_1 \cup \beta_2$ is a basis of V.

\end{proof}